refactor: cleanup and use old memory axiom for demonstration (#31)
* fix: correct filename to fix build

* sync RTypeReader

* working AddOperation.correct again

* migrate all SP1Operations proof

* working AddChip with old/risky memory axiom

SP1Chips/AddChip.lean
@@ -1,4 +1,6 @@
-import SP1Operations
+import SP1Operations.AddOperation
+import SP1Operations.RTypeReader
+import SP1Operations.CPUState
 import LeanRV32D.RiscvInstsEnd
 
 open LeanRV32D.Functions Sail
@@ -7,58 +9,18 @@ namespace AddChip
 
 section constraints
 
-def constraints
-  (Main : Vector BabyBear 23)
-  : SP1ConstraintList :=
+def constraints (Main : Vector BabyBear 23) : SP1ConstraintList :=
   let E0 : BabyBear := Main[22] - 1
-  let E2 : BabyBear := Main[22] * E0
-  let E4 : BabyBear := Main[3] + 4
-  let E6 : BabyBear := 16384 * Main[1]
-  let E8 : BabyBear := E6 + Main[2]
-  [ .assertZero E2
-  ]
-  ++ (AddOperation.constraints #v[Main[11], Main[12], Main[16], Main[17], Main[20], Main[21], Main[22]])
-  ++ (CPUState.constraints
-      { clk_high := Main[0]
-      , clk_16_24 := Main[1]
-      , clk_0_16 := Main[2]
-      , pc := Main[3] }
-      E4
-      4
-      Main[22])
-  ++ (RTypeReader.constraints
-    Main[0]
-    E8
-    -- Main[3]
-    -- 0
-    #v[Main[20], Main[21]]
-    { op_a := Main[4]
-    , op_a_memory :=
-        { prev_value := #v[Main[5], Main[6]]
-        , access_timestamp :=
-            { prev_low := Main[7]
-            , diff_low_limb := Main[8]
-            }
-        }
-    , op_a_0 := Main[9]
-    , op_b := Main[10]
-    , op_b_memory :=
-        { prev_value := #v[Main[11], Main[12]]
-        , access_timestamp :=
-            { prev_low := Main[13]
-            , diff_low_limb := Main[14]
-            }
-        }
-    , op_c := Main[15]
-    , op_c_memory :=
-        { prev_value := #v[Main[16], Main[17]]
-        , access_timestamp :=
-            { prev_low := Main[18]
-            , diff_low_limb := Main[19]
-            }
-        }
-    }
-    Main[22])
+  let E1 : BabyBear := Main[22] * E0
+  let CS0 : List SP1Constraint := AddOperation.constraints #v[Main[11], Main[12]] #v[Main[16], Main[17]] { value := #v[Main[20], Main[21]] } Main[22]
+  let E2 : BabyBear := Main[3] + 4
+  let CS1 : List SP1Constraint := CPUState.constraints { clk_0_16 := Main[2], clk_16_24 := Main[1], clk_high := Main[0], pc := Main[3] } E2 8 Main[22]
+  let E3 : BabyBear := Main[1] * 65536
+  let E4 : BabyBear := Main[2] + E3
+  let CS2 : List SP1Constraint := RTypeReader.constraints Main[0] E4 Main[3] 0 #v[Main[20], Main[21]] { op_a := Main[4], op_a_0 := Main[9], op_a_memory := { access_timestamp := { diff_low_limb := Main[8], prev_low := Main[7] }, prev_value := #v[Main[5], Main[6]] }, op_b := Main[10], op_b_memory := { access_timestamp := { diff_low_limb := Main[14], prev_low := Main[13] }, prev_value := #v[Main[11], Main[12]] }, op_c := Main[15], op_c_memory := { access_timestamp := { diff_low_limb := Main[19], prev_low := Main[18] }, prev_value := #v[Main[16], Main[17]] } } Main[22]
+  [
+    .assertZero E1
+  ] ++ CS0 ++ CS1 ++ CS2
 
 lemma bound_of_constraints (Main : Vector BabyBear 23)
     (cstrs : (constraints Main).allHold)
@@ -70,82 +32,84 @@ lemma bound_of_constraints (Main : Vector BabyBear 23)
   have h_high : Main[21].val < 65536 := add_cstrs.right.right.right
   linarith
 
-lemma toSailM_constraints
-    (Main : Vector BabyBear 23) :
-    (constraints Main).toSailM = (do
-    let _ ← wX_bits (regidx.Regidx (BitVec.ofNat 5 ↑Main[4]))
-      (BitVec.ofNat 32 (↑Main[20] + ↑Main[21] * 65536))
-    let _ ← wX_bits (regidx.Regidx (BitVec.ofNat 5 ↑Main[10]))
-      (BitVec.ofNat 32 (↑Main[11] + ↑Main[12] * 65536))
-    let _ ← wX_bits (regidx.Regidx (BitVec.ofNat 5 ↑Main[15]))
-      (BitVec.ofNat 32 (↑Main[16] + ↑Main[17] * 65536))) := by
-  simp [constraints, SP1ConstraintList.toSailM,
-    AddOperation.constraints, CPUState.constraints, RTypeReader.constraints]
-
 end constraints
 
-def spec_add' (Main : Vector BabyBear 23) : SailM Unit := do
-  let _ ← wX_bits (.Regidx Main[4].1)
-        (BitVec.ofNat 32 (Main[5] + Main[6] * 65536))
-  let _ ← wX_bits (.Regidx Main[10].1)
-    (BitVec.ofNat 32 (Main[11] + Main[12] * 65536))
-  let _ ← execute_RTYPE (.Regidx Main[4].1)
-    (.Regidx Main[10].1) (.Regidx Main[15].val) rop.ADD
+def sp1_add
+  (Main : Vector BabyBear 23)
+  (constraints : (AddChip.constraints Main).allHold)
+  (h_is_real : Main[22] = 1)
+  (rd rs1 rs2 : regidx)
+  : SailM Unit :=
+  let pf : Main[20].val + Main[21].val * 65536 < 2^32 :=
+    by
+      exact bound_of_constraints Main constraints h_is_real
+  do
+    writeReg Register.nextPC (BitVec.addInt (← readReg Register.PC) 4)
+    let rs1_val ← rX_bits rs1
+    let rs2_val ← rX_bits rs2
+    wX_bits rd (BitVec.ofNatLT (Main[20].val + Main[21].val * 65536) pf)
 
-def specAdd (Main : Vector BabyBear 23) : SailM Unit := do
-  let op_a := regidx.Regidx Main[4].val
-  let op_b := regidx.Regidx Main[10].val
-  let op_c := regidx.Regidx Main[15].val
-  let _ ← execute_RTYPE op_a op_b op_c rop.ADD
+def spec_add (rd rs1 rs2 : regidx) : SailM Unit :=
+  do
+    writeReg Register.nextPC (BitVec.addInt (← readReg Register.PC) 4)
+    let _ ← execute_RTYPE rs2 rs1 rd rop.ADD
+    pure ()
 
-theorem SP1Add_Correct (Main : Vector BabyBear 23)
-    (h_constraints : SP1ConstraintList.allHold (constraints Main))
-    (h_is_real : Main[22] = 1)
-    (mstate : PreSail.SequentialState RegisterType trivialChoiceSource)
-    (hmem₁ : mstate.mem[Main[4]]? = some ↑(Main[5] + Main[6] * 65536).val)
-    (hmem₂ : mstate.mem[Main[10]]? = some ↑(Main[11] + Main[12] * 65536).val) :
+theorem sp1_add_implies_spec_add
+  (Main : Vector BabyBear 23)
+  (cstrs : (AddChip.constraints Main).allHold)
+  (h_is_real : Main[22] = 1)
+  (rd rs1 rs2 : regidx)
+  (read_b : rX_bits rs1 = pure (BitVec.ofNat 32 (Main[11].val + Main[12].val * 65536)))
+  (read_b_range : Main[11] < 65536 ∧ Main[12] < 65536)
+  (read_c : rX_bits rs2 = pure (BitVec.ofNat 32 (Main[16].val + Main[17].val * 65536)))
+  (read_c_range : Main[16] < 65536 ∧ Main[17] < 65536)
+  :
+  let res := (sp1_add Main cstrs h_is_real rd rs1 rs2).run s
+  let res_spec := (spec_add rd rs1 rs2).run s
+  res = res_spec :=
+  by
+    simp [sp1_add, spec_add, EStateM.run]
+    simp [execute_RTYPE]
 
-    let sp1Add : SailM Unit := (constraints Main).toSailM
-    sp1Add.run mstate = (specAdd Main).run mstate := by
-  sorry
+    simp [SP1ConstraintList.allHold] at cstrs
+    simp [constraints] at cstrs
+    obtain ⟨orig_cstrs, ⟨add_cstrs, ⟨cpu_strs, adapter_cstrs⟩⟩⟩ := cstrs
 
-theorem sp1_add_eq_spec_add
-    (Main : Vector BabyBear 23)
-    (cstrs : SP1ConstraintList.allHold (constraints Main))
-    (h_is_real : Main[22] = 1) :
-    (constraints Main).toSailM = spec_add' Main := by
-  unfold spec_add'
-  rw [toSailM_constraints]
+    -- Poor man's "coercion"
+    let M11_U16 : U16 := ⟨Main[11], read_b_range.left⟩
+    let M12_U16 : U16 := ⟨Main[12], read_b_range.right⟩
+    let M16_U16 : U16 := ⟨Main[16], read_c_range.left⟩
+    let M17_U16 : U16 := ⟨Main[17], read_c_range.right⟩
+    let M22_U1  : U1  := ⟨Main[22], by simp [h_is_real]⟩
 
-  let spare_cstrs := cstrs
-  -- Extract the various constraints from the assumption
-  simp [constraints] at cstrs
-  obtain ⟨orig_cstrs, ⟨add_cstrs, ⟨cpu_strs, adapter_cstrs⟩⟩⟩ := cstrs
-  rw [h_is_real] at adapter_cstrs add_cstrs
+    let add_spec_wo_proof :=
+      AddOperation.correct'
+        #v[M11_U16, M12_U16]
+        #v[M16_U16, M17_U16]
+        { value := #v[Main[20], Main[21]] }
+        M22_U1
+        (by aesop)
+        (by aesop)
+    simp [AddOperation.constraints, SP1Constraint.toProp, h_is_real, ByteOpcode.ofNat, Nat.ble, Nat.beq, ByteOpcode.constrain] at add_cstrs
+    have h_low  : Main[20].val < 65536 := add_cstrs.right.right.left
+    have h_high : Main[21].val < 65536 := add_cstrs.right.right.right
+    have h_res_is_u16 : Main[20].val + Main[21].val * 65536 < 2^32 := by clear * - h_low h_high; linarith
+    let add_spec := add_spec_wo_proof h_res_is_u16
+    simp [AddOperation.value, Word.toBV32_U16] at add_spec
+    rw [add_spec]
 
-  -- The `RTypeReader` gives bounds on the size of previous memory values
-  let op_b_memory_bound := RTypeReader.op_b_memory_lt_of_constraints adapter_cstrs
-  let op_c_memory_bound := RTypeReader.op_c_memory_lt_of_constraints adapter_cstrs
+    rw [read_b, read_c, pure_bind, pure_bind]
+    rw [pure_bind, pure_bind]
 
-  -- Bounded representations of the input limbs
-  let M11_U16 : U16 := ⟨Main[11], op_b_memory_bound.1⟩
-  let M12_U16 : U16 := ⟨Main[12], op_b_memory_bound.2⟩
-  let M16_U16 : U16 := ⟨Main[16], op_c_memory_bound.1⟩
-  let M17_U16 : U16 := ⟨Main[17], op_c_memory_bound.2⟩
-  let M22_U1  : U1  := ⟨Main[22], by aesop⟩
-  have hb1 : Main[11].val + Main[12].val * 65536 < 2 ^ 32 := by
-    have := M11_U16.in_range; have := M12_U16.in_range; linarith
-  have hb2 : Main[16].val + Main[17].val * 65536 < 2 ^ 32 := by
-    have := M16_U16.in_range; have := M17_U16.in_range; linarith
-
-  simp [constraints, SP1ConstraintList.toSailM]
-  simp [execute_RTYPE]
-
-  have := AddOperation.correct' Main[20] Main[21] M11_U16 M12_U16 M16_U16 M17_U16 add_cstrs
-
-  rw [← BitVec.ofNatLT_eq_ofNat (bound_of_constraints Main spare_cstrs h_is_real)]
-  rw [this]
-
-  sorry
-
-end AddChip
+    let h_b_is_u16 : Main[11].val + Main[12].val * 65536 < 2^32 :=
+      by
+        clear * - read_b_range
+        simp [Fin.lt_def] at *
+        linarith
+    let h_c_is_u16 : Main[16].val + Main[17].val * 65536 < 2^32 :=
+      by
+        clear * - read_c_range
+        simp [Fin.lt_def] at *
+        linarith
+    rw [←BitVec.ofNatLT_eq_ofNat h_b_is_u16, ←BitVec.ofNatLT_eq_ofNat h_c_is_u16]
