SP1Operations/AddOperation.lean
@@ -1,117 +1,141 @@
 import SP1Foundations
 
+structure AddOperation (T : Type) where
+  value : Word T
+
+instance coe [Coe A B] : Coe (AddOperation A) (AddOperation B) where
+  coe w := { value := w.value }
+
 namespace AddOperation
 
 def constraints
-  (I : Vector BabyBear 7)
+  (a : Word BabyBear)
+  (b : Word BabyBear)
+  (cols : AddOperation BabyBear)
+  (is_real : BabyBear)
   : SP1ConstraintList :=
-  let E0 := I[6] - 1
-  let E2 := I[6] * E0
-  let E4 := I[0] + I[2]
-  let E6 := E4 - I[4]
-  let E8 := E6 + 0
-  let E10 := E8 * 2013235201
-  let E12 := E10 - 1
-  let E14 := E10 * E12
-  let E16 := I[6] * E14
-  let E18 := I[1] + I[3]
-  let E20 := E18 - I[5]
-  let E22 := E20 + E10
-  let E24 := E22 * 2013235201
-  let E26 := E24 - 1
-  let E28 := E24 * E26
-  let E30 := I[6] * E28
-  [ .assertZero E2
-  , .assertZero E16
-  , .assertZero E30
-  , .send (.byte (ByteOpcode.ofNat 6) I[4] 16 0) I[6]
-  , .send (.byte (ByteOpcode.ofNat 6) I[5] 16 0) I[6]
+  let E0 : BabyBear := is_real - 1
+  let E1 : BabyBear := is_real * E0
+  let E2 : BabyBear := a[0] + b[0]
+  let E3 : BabyBear := E2 - cols.value[0]
+  let E4 : BabyBear := E3 + 0
+  let E5 : BabyBear := E4 * 2013235201
+  let E6 : BabyBear := E5 - 1
+  let E7 : BabyBear := E5 * E6
+  let E8 : BabyBear := is_real * E7
+  let E9 : BabyBear := a[1] + b[1]
+  let E10 : BabyBear := E9 - cols.value[1]
+  let E11 : BabyBear := E10 + E5
+  let E12 : BabyBear := E11 * 2013235201
+  let E13 : BabyBear := E12 - 1
+  let E14 : BabyBear := E12 * E13
+  let E15 : BabyBear := is_real * E14
+  [
+    .assertZero E1,
+    .assertZero E8,
+    .assertZero E15,
+    .send (.byte (ByteOpcode.ofNat 6) cols.value[0] 16 0) is_real,
+    .send (.byte (ByteOpcode.ofNat 6) cols.value[1] 16 0) is_real
   ]
 
--- Should we be including the bounds at this level? Instead done below seperately
-def spec
-  (a0 a1 : U16)
-  (b0 b1 : U16)
-  (c0 c1 : U16)
-  (is_real : U1) : Prop :=
-    is_real = 1 → BitVec.ofU16 a0 a1 = BitVec.ofU16 b0 b1 + BitVec.ofU16 c0 c1
-
 def constraintsProp
-  (I : Vector BabyBear 7) : Prop :=
+  (a : Word BabyBear)
+  (b : Word BabyBear)
+  (cols : AddOperation BabyBear)
+  (is_real : BabyBear)
+  : Prop :=
   let carry0  : BabyBear := 0
-  let carry1  : BabyBear := (I[0] + I[2] - I[4] + carry0) * (baseInv : BabyBear)
-  let carry2  : BabyBear := (I[1] + I[3] - I[5] + carry1) * (baseInv : BabyBear)
-  I[6] = 0 ∨ (
-    I[6] = 1 ∧
+  let carry1  : BabyBear := (a[0] + b[0] - cols.value[0] + carry0) * (baseInv : BabyBear)
+  let carry2  : BabyBear := (a[1] + b[1] - cols.value[1] + carry1) * (baseInv : BabyBear)
+  is_real = 0 ∨ (
+    is_real = 1 ∧
     (carry1 = 0 ∨ carry1 = 1) ∧
     (carry2 = 0 ∨ carry2 = 1) ∧
-    (I[4] < 65536) ∧
-    (I[5] < 65536)
+    (cols.value[0] < 65536) ∧
+    (cols.value[1] < 65536)
   )
 
 def constraints_iff_constraintsProp
-  (I : Vector BabyBear 7) : (constraints I).allHold ↔ constraintsProp I := by
-  by_cases h : I[6] = 0
+  (a : Word BabyBear)
+  (b : Word BabyBear)
+  (cols : AddOperation BabyBear)
+  (is_real : BabyBear)
+  : (constraints a b cols is_real).allHold ↔ constraintsProp a b cols is_real := by
+  by_cases h : is_real = 0
   · simp [constraints, constraintsProp, h]
-  · by_cases h' : I[6] = 1 <;> simp [constraints, constraintsProp, h, h', sub_eq_zero]
+  · by_cases h' : is_real = 1 <;> simp [constraints, constraintsProp, h, h', sub_eq_zero]
+
+-- Should we be including the bounds at this level? Instead done below seperately
+def spec
+  (a b : Word U16)
+  (cols : AddOperation U16)
+  (is_real : U1) : Prop :=
+    is_real = 1 → cols.value.toBV32_U16 = a.toBV32_U16 + b.toBV32_U16
 
 theorem correct
-  (a0 a1 b0 b1 c0 c1 : U16)
+  (a b : Word U16)
+  (cols : AddOperation U16)
   (is_real : U1) :
-    (constraints #v[b0, b1, c0, c1, a0, a1, is_real]).allHold →
-    spec a0 a1 b0 b1 c0 c1 is_real := by
-  rw [constraints_iff_constraintsProp (#v[b0, b1, c0, c1, a0, a1, is_real])]
-  simp [constraintsProp, spec]
-  intro q1
+    (constraints a b cols is_real).allHold →
+    spec a b cols is_real := by
+      rw [constraints_iff_constraintsProp a b cols is_real]
+      simp [constraintsProp, spec]
+      intro q1
 
-  intro h_is_real
-  simp [h_is_real] at q1
+      intro h_is_real
+      simp [h_is_real] at q1
 
-  let ⟨qq1, ⟨qq2, ⟨qq3, aa4⟩⟩⟩ := q1
-  clear q1
-  simp [sub_eq_zero, mul_eq_zero] at qq1 qq2
-  simp [BitVec.ofU16, BitVec.ofNatLT]
+      let ⟨qq1, ⟨qq2, ⟨qq3, aa4⟩⟩⟩ := q1
+      clear q1
+      simp [sub_eq_zero, mul_eq_zero] at qq1 qq2
+      simp [Word.toBV32_U16, BitVec.ofNatLT]
 
-  cases qq1 with
-  | inl qqq1 =>
-      rw [qqq1] at qq2
-      simp [Fin.mul_def, Fin.sub_def, Fin.add_def, Fin.ext_iff, BabyBearPrime] at *
-      rw [Fin.lt_def] at qq3 aa4
-      aesop (add 50% tactic (by omega))
-  | inr qqq1 =>
-      rw [qqq1] at qq2
-      simp [Fin.mul_def, Fin.sub_def, Fin.add_def, Fin.ext_iff, BabyBearPrime] at *
-      rw [Fin.lt_def] at qq3 aa4
-      aesop (add 50% tactic (by omega))
+      cases qq1 with
+      | inl qqq1 =>
+          rw [qqq1] at qq2
+          simp [Fin.mul_def, Fin.sub_def, Fin.add_def, Fin.ext_iff, BabyBearPrime] at *
+          simp [Fin.lt_def] at qq3 aa4
+          aesop (add 50% tactic (by omega))
+      | inr qqq1 =>
+          rw [qqq1] at qq2
+          simp [Fin.mul_def, Fin.sub_def, Fin.add_def, Fin.ext_iff, BabyBearPrime] at *
+          simp [Fin.lt_def] at qq3 aa4
+          aesop (add 50% tactic (by omega))
 
 open BitVec
 
-lemma lt_of_constraintsAllHold {c0 c1 a0 a1 b0 b1 : BabyBear}
-    (h : (constraints #v[c0, c1, b0, b1, a0, a1, 1]).allHold) : a0 < 65536 := by
+lemma lt_of_constraintsAllHold
+    (h : (constraints a b cols is_real).allHold)
+    (h_is_real : is_real = 1) : cols.value[0] < 65536 := by
   rw [constraints_iff_constraintsProp] at h
   rw [constraintsProp] at h
   simp at h
+  subst h_is_real
   tauto
 
-lemma lt_of_constraintsAllHold' {c0 c1 a0 a1 b0 b1 : BabyBear}
-    (h : (constraints #v[c0, c1, b0, b1, a0, a1, 1]).allHold) : a1 < 65536 := by
+lemma lt_of_constraintsAllHold'
+    (h : (constraints a b cols is_real).allHold)
+    (h_is_real : is_real = 1) : cols.value[1] < 65536 := by
   rw [constraints_iff_constraintsProp] at h
   rw [constraintsProp] at h
   simp at h
+  subst h_is_real
   tauto
 
 /-- Version of correctness using specific bitvecs.
 To get good rewrites we allow arbitrary proofs on the left (should do the reverse for ← rw to work)-/
-lemma correct' (c0 c1 : BabyBear) (a0 a1 b0 b1 : U16)
-    (h : (constraints #v[a0, a1, b0, b1, c0, c1, 1]).allHold)
-    (pf : c0.val + c1.val * 65536 < 2 ^ 32) :
-    (c0.val + c1.val * 65536)#'pf =
-      (BitVec.ofU16 a0 a1 + BitVec.ofU16 b0 b1) := by
-  let c0' : U16 := ⟨c0, lt_of_constraintsAllHold h⟩
-  let c1' : U16 := ⟨c1, lt_of_constraintsAllHold' h⟩
-  refine correct c0' c1' a0 a1 b0 b1 1 ?_ rfl
-  exact h
-
-
+lemma correct'
+    (a b : Word U16)
+    (cols : AddOperation BabyBear)
+    (is_real : U1)
+    (h : (constraints a b cols is_real).allHold)
+    (h_is_real : is_real = 1)
+    (pf : cols.value[0].val + cols.value[1].val * 65536 < 2 ^ 32) :
+    (cols.value[0].val + cols.value[1].val * 65536)#'pf =
+      (a.toBV32_U16 + b.toBV32_U16) := by
+  -- TODO(gzgz): don't use aesop
+  let c0' : U16 := ⟨cols.value[0], lt_of_constraintsAllHold h (by aesop)⟩
+  let c1' : U16 := ⟨cols.value[1], lt_of_constraintsAllHold' h (by aesop)⟩
+  refine correct a b { value := #v[c0', c1'] } is_real h h_is_real
 
 end AddOperation
