SP1Operations.lean
@@ -1,7 +1,7 @@
 import SP1Operations.ALUTypeReader
 import SP1Operations.Add4Operation
 import SP1Operations.AddOperation
-import SP1Operations.BitWiseU16Operation
+import SP1Operations.BitwiseU16Operation
 import SP1Operations.BitwiseOperation
 import SP1Operations.CPUState
 import SP1Operations.IsZeroOperation
@@ -10,5 +10,5 @@ import SP1Operations.MSBOperation
 import SP1Operations.MemoryConsistency
 import SP1Operations.RTypeReader
 import SP1Operations.SubOperation
-import SP1Operations.U16ToU8OperationSafe
--- import SP1Operations.U16ToU8OperationUnsafe
+import SP1Operations.U16toU8OperationSafe
+import SP1Operations.U16toU8OperationUnsafe
